Bet/README.md
@@ -1,5 +1,5 @@
 
-To build, run `zebra  --z3rlimit 3500000 -c Bet.fst`.  
+To build, run `zebra  --z3rlimit 3000000 -c Bet.fst`.  
 To run tests, run
 ```
 zebra -r Tests/Buy.fsx
